src/Prelude.thy
@@ -4,17 +4,20 @@ definition from_to :: "nat \<Rightarrow> nat \<Rightarrow> nat list" where
 "from_to x y = upt x (Suc y)"
 
 
-definition maps_as_map :: "('a,'b) map set \<Rightarrow> ('a,'b) map \<Rightarrow> bool" where
-"maps_as_map ms m = (
+definition maps_to_map_prop :: "('a,'b) map set \<Rightarrow> ('a,'b) map \<Rightarrow> bool" where
+"maps_to_map_prop ms m = (
 (! a b. (m a = Some b) = (? m' : ms. m' a = Some b)) &
 (! a. (m a = None) = (! m' : ms. m' a = None))
 )"
 
-definition merge_maps :: "('a,'b) map set \<Rightarrow> ('a,'b) map" where
-"merge_maps ms = (SOME m. maps_as_map ms m)"
+definition maps_to_map :: "('a,'b) map set \<Rightarrow> ('a,'b) map" where
+"maps_to_map ms = (SOME m. maps_to_map_prop ms m)"
 
-lemma "maps_as_map ms (merge_maps ms)"
+lemma "maps_to_map_prop ms (maps_to_map ms)"
   apply(force intro:FIXME)
   done
+
+definition leaves_to_map :: "('k * 'v) list list \<Rightarrow> ('k,'v) map" where
+"leaves_to_map ls = (image map_of (set ls)) |> maps_to_map"
 
 end
