src/Tree_stack.thy
@@ -1,13 +1,13 @@
 theory Tree_stack imports Tree begin
 
-(* the bound is a bound on ALL children, not just rs!i *)
-datatype cnode_t = Cnode "node_t * nat * bound_t"  (* n,i,b *)
+(* the bound l,u is a bound on ALL children, not just rs!i; l,u could be calculated from the ts *)
+datatype cnode_t = Cnode "key option * key list * Tree list * nat * key option"  (* l,ks,rs,i,u *)
 
 
-definition dest_cnode_t :: "cnode_t \<Rightarrow> node_t * nat * bound_t" where
-"dest_cnode_t c = (case c of Cnode (n,i,b) \<Rightarrow> (n,i,b))"
+definition dest_cnode_t :: "cnode_t \<Rightarrow> key option * key list * Tree list * nat * key option" where
+"dest_cnode_t c = (case c of Cnode (l,ks,rs,i,u) \<Rightarrow> (l,ks,rs,i,u))"
 
-lemma dest_cnode_t_def_2: "dest_cnode_t (Cnode(n,i,b)) = (n,i,b)"
+lemma dest_cnode_t_def_2: "dest_cnode_t (Cnode(l,ks,rs,i,u)) = (l,ks,rs,i,u)"
 apply(simp add: dest_cnode_t_def)
 done
 
@@ -17,6 +17,18 @@ type_synonym context_t = "cnode_t list"
 type_synonym tree_stack_t = "cnode_t list"
 
 
+(* search_key_to_index ------ *)
+
+(*tr: assumes xs are sorted; returns list length if not found*)
+(*begin search key to index definition *)
+definition search_key_to_index :: "key list => key => nat" where
+"search_key_to_index ks k = (
+let num_keys = length ks in
+let i = List.find (% x. key_lt k (ks!x)) (upt 0 num_keys) in
+let i' = (case i of None => num_keys | Some x => x) in
+i')"
+(*end search key to index definition *)
+
 
 
 (* bound from cnode ---------------------------------------- *)
@@ -24,9 +36,8 @@ type_synonym tree_stack_t = "cnode_t list"
 (* make sure we use the existing bound in case i is extremal *)
 definition cnode_to_bound :: "cnode_t \<Rightarrow> bound_t" where
 "cnode_to_bound cn = (
-  let (n,i,b) = dest_cnode_t cn in
-  let (ks,rs) = n in
-  index_to_bound ks i |> with_parent_bound b)"
+  let (l,ks,rs,i,u) = dest_cnode_t cn in
+  index_to_bound ks i |> with_parent_bound (l,u))"
 
 
 
@@ -35,14 +46,12 @@ definition cnode_to_bound :: "cnode_t \<Rightarrow> bound_t" where
 
 
 (* FIXME adjust scala defns *)      
-definition wellformed_cnode :: "ms_t => cnode_t => bool " where
-"wellformed_cnode ms cn = (
-  let (n1,i1,x1) = dest_cnode_t cn in 
-  let (l1,u1) = x1 in
-  let (ks,rs) = n1 in
+definition wellformed_cnode :: "key \<Rightarrow> ms_t => cnode_t => bool " where
+"wellformed_cnode k0 ms cn = (
+  let (l,ks,rs,i,u) = dest_cnode_t cn in 
   let b1 = wellformed_tree ms (Node(ks,rs)) in  (* FIXME wellformed_kv_tree *)
-  let b2 = i1 : set(subtree_indexes (ks,rs)) in
-  let b3 = check_keys l1 (keys (Node(ks,rs))) u1 in
+  let b2 = search_key_to_index ks k0 = i in
+  let b3 = check_keys l (set (keys (Node(ks,rs)))) u in
   b1&b2&b3)
 "
 
@@ -60,16 +69,37 @@ lemma ts_to_ms_def_2: "
   done
 
 
-fun wellformed_context :: "context_t => bool" where
-"wellformed_context xs = (
+fun wellformed_context :: "key \<Rightarrow> tree_stack_t => bool" where
+"wellformed_context k0 xs = (
   case xs of Nil \<Rightarrow> True
-  | cn#cns \<Rightarrow> (wellformed_cnode (ts_to_ms cns) cn & wellformed_context cns))"
+  | cn#cns \<Rightarrow> (wellformed_cnode k0 (ts_to_ms cns) cn & wellformed_context k0 cns))"
 (*end wfcontext definition*)
 
 lemma wellformed_context_def_2: "
-  (wellformed_context  Nil = True) &
-  (wellformed_context (cn#cns) = (wellformed_cnode (ts_to_ms cns) cn & wellformed_context cns))"
+  (wellformed_context k0 Nil = True) &
+  (wellformed_context k0 (cn#cns) = (wellformed_cnode k0 (ts_to_ms cns) cn & wellformed_context k0 cns))"
 by simp
+
+
+(* stack reassembly ----------------------------------- *)
+
+fun reass :: "Tree \<Rightarrow> tree_stack_t \<Rightarrow> Tree" where
+"reass t ts = (
+  case ts of
+  Nil \<Rightarrow> t
+  | cn#cns \<Rightarrow> (
+    let (l,ks,rs,i,u) = dest_cnode_t cn in
+    let t2 = Node(ks,rs[i:=t]) in
+    reass t2 cns
+))"
+
+
+(* lemmas ------------------------------------------------ *)
+
+definition lemma_reass_1 :: bool where
+"lemma_reass_1 = (! ts t.
+  ? xs zs. (reass t ts) |> tree_to_leaves = xs@(tree_to_leaves t)@zs)"
+
 
 
 end
