src/Key_value_proof.thy
@@ -5,14 +5,6 @@ begin
 (* FIXME most of these lemmas should be unnecessary - they are all solvable with 1st order proof *)
 
 
-(* FIXME might like to use strict total order with key_lt and aim to always eliminate key_le - better automation *)
-definition total_order_key_lte :: " bool" where
-"total_order_key_lte == (\<forall> a b c. 
-   (key_le a b \<and> key_le b a \<longrightarrow> key_eq a b) \<and>
-   (key_le a b \<and> key_le b c \<longrightarrow> key_le a c) \<and>
-   (key_le a b \<or> key_le b a)
-\<and> (a = b \<longrightarrow> (key_le a b)))" (* FIXME just use defn of key_le, with = *)
-
 lemma neg_key_lt: "! a b. total_order_key_lte \<longrightarrow> (~ key_lt a b) = (key_le b a)"
 apply rule+
 apply (unfold total_order_key_lte_def)
